theories/zoo_saturn/mpsc_queue_2__opaque.v
@@ -1,7 +1,0 @@
-Require Import zoo_saturn.mpsc_queue_2__code.
-
-#[global] Opaque mpsc_queue_2٠create.
-#[global] Opaque mpsc_queue_2٠is_empty.
-#[global] Opaque mpsc_queue_2٠push_front.
-#[global] Opaque mpsc_queue_2٠push_back.
-#[global] Opaque mpsc_queue_2٠pop.
