theories/zoo_saturn/queue_mpsc_2__code.v
@@ -5,40 +5,40 @@ Require Import zoo_std.domain.
 Require Import zoo_std.glist.
 Require Import zoo.options.
 
-Notation "'mpsc_queue_2٠front'" := (
-  in_type "zoo_saturn.mpsc_queue_2.t" 0
+Notation "'queue_mpsc_2٠front'" := (
+  in_type "zoo_saturn.queue_mpsc_2.t" 0
 )(in custom zoo_field
 ).
-Notation "'mpsc_queue_2٠back'" := (
-  in_type "zoo_saturn.mpsc_queue_2.t" 1
+Notation "'queue_mpsc_2٠back'" := (
+  in_type "zoo_saturn.queue_mpsc_2.t" 1
 )(in custom zoo_field
 ).
 
-Definition mpsc_queue_2٠create : val :=
+Definition queue_mpsc_2٠create : val :=
   𝗳𝘂𝗻 ⎽ ->
     { §glist٠Nil, §glist٠Nil }.
 
-Definition mpsc_queue_2٠is_empty : val :=
+Definition queue_mpsc_2٠is_empty : val :=
   𝗳𝘂𝗻 "t" ->
-    𝗺𝗮𝘁𝗰𝗵 "t".{mpsc_queue_2٠front} 𝘄𝗶𝘁𝗵
+    𝗺𝗮𝘁𝗰𝗵 "t".{queue_mpsc_2٠front} 𝘄𝗶𝘁𝗵
     | glist٠Cons ⎽ ⎽ ->
         false
     | glist٠Nil ->
-        "t".{mpsc_queue_2٠back} == §glist٠Nil
+        "t".{queue_mpsc_2٠back} == §glist٠Nil
     𝗲𝗻𝗱.
 
-Definition mpsc_queue_2٠push_front : val :=
+Definition queue_mpsc_2٠push_front : val :=
   𝗳𝘂𝗻 "t" "v" ->
-    "t" <-{mpsc_queue_2٠front}
-      ‘glist٠Cons[ "v", "t".{mpsc_queue_2٠front} ].
+    "t" <-{queue_mpsc_2٠front}
+      ‘glist٠Cons[ "v", "t".{queue_mpsc_2٠front} ].
 
-Definition mpsc_queue_2٠push_back : val :=
+Definition queue_mpsc_2٠push_back : val :=
   𝗿𝗲𝗰 "push_back" "t" "v" ->
-    𝗹𝗲𝘁 "back" = "t".{mpsc_queue_2٠back} 𝗶𝗻
+    𝗹𝗲𝘁 "back" = "t".{queue_mpsc_2٠back} 𝗶𝗻
     𝗶𝗳
       ~
       𝗰𝗮𝘀
-        "t".[mpsc_queue_2٠back]
+        "t".[queue_mpsc_2٠back]
         "back"
         ‘glist٠Cons[ "v", "back" ]
     𝘁𝗵𝗲𝗻 (
@@ -46,20 +46,20 @@ Definition mpsc_queue_2٠push_back : val :=
       "push_back" "t" "v"
     ).
 
-Definition mpsc_queue_2٠pop : val :=
+Definition queue_mpsc_2٠pop : val :=
   𝗳𝘂𝗻 "t" ->
-    𝗺𝗮𝘁𝗰𝗵 "t".{mpsc_queue_2٠front} 𝘄𝗶𝘁𝗵
+    𝗺𝗮𝘁𝗰𝗵 "t".{queue_mpsc_2٠front} 𝘄𝗶𝘁𝗵
     | glist٠Nil ->
         𝗺𝗮𝘁𝗰𝗵
-          glist٠rev (𝘅𝗰𝗵𝗴 "t".[mpsc_queue_2٠back] §glist٠Nil)
+          glist٠rev (𝘅𝗰𝗵𝗴 "t".[queue_mpsc_2٠back] §glist٠Nil)
         𝘄𝗶𝘁𝗵
         | glist٠Nil ->
             §None
         | glist٠Cons "v" "front" ->
-            "t" <-{mpsc_queue_2٠front} "front" ⍮
+            "t" <-{queue_mpsc_2٠front} "front" ⍮
             ‘Some( "v" )
         𝗲𝗻𝗱
     | glist٠Cons "v" "front" ->
-        "t" <-{mpsc_queue_2٠front} "front" ⍮
+        "t" <-{queue_mpsc_2٠front} "front" ⍮
         ‘Some( "v" )
     𝗲𝗻𝗱.
