theories/zoo_saturn/queue_mpsc_2__opaque.v
@@ -1,0 +1,7 @@
+Require Import zoo_saturn.queue_mpsc_2__code.
+
+#[global] Opaque queue_mpsc_2٠create.
+#[global] Opaque queue_mpsc_2٠is_empty.
+#[global] Opaque queue_mpsc_2٠push_front.
+#[global] Opaque queue_mpsc_2٠push_back.
+#[global] Opaque queue_mpsc_2٠pop.
