theories/zoo_saturn/queue_mpsc_2__types.v
@@ -6,10 +6,10 @@ Require Export zoo_std.glist.
 Require Import zoo.options.
 
 Notation "'front'" := (
-  in_type "zoo_saturn.mpsc_queue_2.t" 0
+  in_type "zoo_saturn.queue_mpsc_2.t" 0
 )(in custom zoo_field
 ).
 Notation "'back'" := (
-  in_type "zoo_saturn.mpsc_queue_2.t" 1
+  in_type "zoo_saturn.queue_mpsc_2.t" 1
 )(in custom zoo_field
 ).
